Generalize requirement patterns and add proofs for Smart lighting program

Pattern2_Def.thy
@@ -2,29 +2,42 @@ theory Pattern2_Def
   imports Pattern3_Def
 begin
 
-definition P2all where " P2all s A \<equiv>
+definition previous_all where " previous_all s A \<equiv>
 \<forall> s1. consecutive s1 s \<longrightarrow> A s1"
 
-definition P2ex where "P2ex s A \<equiv>
+definition previous_ex where "previous_ex s A \<equiv>
 \<exists> s1. consecutive s1 s \<and> A s1"
 
-definition P2 where  "P2 s A1 A2 \<equiv> toEnvP s \<and>
-(\<forall> s1 s2. consecutive s1 s2 \<and> substate s2 s \<and> A1 s1 s2 \<longrightarrow> A2 s1 s2)"
+definition always2 where  "always2 s A1 A2 \<equiv> 
+\<forall> s1 s2. substate s1 s2 \<and> substate s2 s \<and> toEnvP s1 \<and> toEnvP s2 \<and> toEnvNum s1 s2 = 1 \<and> A1 s1 s2 \<longrightarrow> A2 s2"
 
-lemma P2all_rule: "consecutive s0 s \<Longrightarrow>  A s0 \<Longrightarrow> P2all s A"
-  apply(unfold  P2all_def)
+lemma previous_all_one_point: "consecutive s0 s \<Longrightarrow>  A s0 \<Longrightarrow> previous_all s A"
+  apply(unfold  previous_all_def)
   apply simp
   by (metis toEnvNum_eq_imp_eq2)
 
-lemma P2ex_rule: "consecutive s0 s \<Longrightarrow>  A s0  \<Longrightarrow> P2ex s A"
-  apply(unfold  P2ex_def)
+lemma previous_ex_one_point: "consecutive s0 s \<Longrightarrow>  A s0  \<Longrightarrow> previous_ex s A"
+  apply(unfold  previous_ex_def)
   by auto
 
-lemma P2_rule: "consecutive s0 s \<Longrightarrow> P2 s0 A1 A2 \<Longrightarrow> (consecutive s0 s \<Longrightarrow> A1 s0 s \<longrightarrow> A2 s0 s) \<Longrightarrow> P2 s A1 A2"
-  apply simp
-  apply(unfold P2_def)
-  apply simp
-  by (metis One_nat_def substate_noteq_imp_substate_of_pred toEnvNum_eq_imp_eq2)
+lemma previous_all_rule: "
+(\<forall> s1. toEnvP s1 \<and> substate s1 s0 \<and> A s1 \<longrightarrow> A' s1) \<Longrightarrow>
+(\<forall> s1. toEnvP s1 \<and> substate s1 s0 \<and> previous_all s1 A  \<longrightarrow> previous_all s1 A')"
+  apply(unfold previous_all_def)
+  by (meson consecutive.simps substate_trans)
+
+lemma previous_ex_rule: "
+(\<forall> s1. toEnvP s1 \<and> substate s1 s \<and> A s1 \<longrightarrow> A' s1) \<Longrightarrow>
+(\<forall> s1. toEnvP s1 \<and> substate s1 s \<and> previous_ex s1 A  \<longrightarrow> previous_ex s1 A')"
+  apply(unfold previous_ex_def)
+  by (meson consecutive.simps substate_trans)
+
+lemma always2_rule: "consecutive s0 s \<Longrightarrow>
+always2 s0 A1 A2 \<and> (\<not> A1 s0 s \<or> A2' s) \<and> (\<forall> s1. toEnvP s1 \<and> substate s1 s0 \<and> A2 s1 \<longrightarrow> A2' s1) \<Longrightarrow> always2 s A1 A2'"
+  apply(unfold always2_def)
+  by (metis consecutive.elims(2) substate_noteq_imp_substate_of_pred toEnvNum_eq_imp_eq2)
+
+lemma always2_einv2req: "always2 s A1 A2 \<and>  (\<forall> s1. toEnvP s1 \<and> substate s1 s \<and> A2 s1 \<longrightarrow> A2' s1) \<Longrightarrow> always2 s A1 A2'"
+  using always2_def by auto
 
 end
-  
