Pattern3_Def.thy
@@ -1,14 +1,20 @@
 theory Pattern3_Def
-  imports VCTheoryLemmas
+  imports RequirementLemmas
 begin
 
-definition P3 where "P3 s A1 A2 \<equiv>
-\<forall> s1. substate s1 s \<and> toEnvP s1 \<and> A1 s1 \<longrightarrow> A2 s1"
+definition always where "always s A \<equiv>
+\<forall> s1. substate s1 s \<and> toEnvP s1 \<and> A s1"
 
-lemma P3_rule: "P3 s0 A1 A2 \<Longrightarrow> (A1 s \<longrightarrow> A2 s) \<Longrightarrow> toEnvP s0 \<and>  toEnvP s \<and> substate s0 s \<and> toEnvNum s0 s = 1 \<Longrightarrow> P3 s A1 A2"
-  apply(unfold P3_def)
-  using substate_noteq_imp_substate_of_pred by blast
+lemma always_rule: "always s0 A \<and> (A' s) \<and> (\<forall> s1 . toEnvP s1 \<and> substate s1 s0 \<and>A s1 \<longrightarrow> A' s1) \<Longrightarrow>
+consecutive s0 s \<Longrightarrow> always s A'"
+  apply(unfold always_def)
+  using substate_antisym by auto
 
-
+lemma always_einv2req: " always s A \<and>  (\<forall> s1 . toEnvP s1 \<and> substate s1 s \<and>A s1 \<longrightarrow> A' s1) \<Longrightarrow>
+  always s A'"
+  apply(unfold always_def)
+  by simp
 
 end
+  
+     
