Pattern5_Def.thy
@@ -1,5 +1,5 @@
 theory Pattern5_Def
-  imports VCTheoryLemmas
+  imports Pattern2_Def
 begin
 
 definition P5inv where "P5inv s t t1 A1 A2 \<equiv>
@@ -91,6 +91,106 @@ lemma P5_1_einv2req: "P5_1inv s t t1 A1 A2 \<Longrightarrow> P5_1 s t A1 A2"
   apply auto
   done
 
+definition constrained_always where "constrained_always s1 s t A \<equiv>
+\<forall> s2. toEnvP s2 \<and> substate s1 s2 \<and> substate s2 s \<and> toEnvNum s1 s2 < t \<longrightarrow> A s2"
+
+definition constrained_always_inv where "constrained_always_inv s1 s t t1 A \<equiv>
+t = 0 \<or>toEnvNum s1 s \<ge> t1 \<and>
+(\<forall> s2. toEnvP s2 \<and> substate s1 s2 \<and> substate s2 s \<and> toEnvNum s1 s2 < t \<longrightarrow> A s2)"
+
+lemma constrained_always_rule: "consecutive s0 s \<Longrightarrow>
+t = 0 \<or> (\<forall> s1. toEnvP s1 \<and> substate s1 s0 \<and> A s1 \<longrightarrow> A' s1) \<and>
+(t1 + 1 \<ge> t \<or> A' s) \<and> t1' \<le> t1 + 1 \<Longrightarrow>
+(\<forall> s1. toEnvP s1 \<and> substate s1 s0 \<and> constrained_always_inv s1 s0 t t1 A \<longrightarrow> constrained_always_inv s1 s t t1' A')"
+  apply(unfold constrained_always_inv_def)
+  apply(cases "t = 0")
+   apply simp_all
+  by (smt (verit) One_nat_def Suc_eq_plus1 dual_order.trans leD not_less_eq_eq substate_noteq_imp_substate_of_pred toEnvNum3)
+
+lemma constrained_always_one_point: "t = 0 \<or> t1 = 0 \<and> ( A s) \<Longrightarrow> constrained_always_inv s s t t1 A"
+  apply(unfold constrained_always_inv_def)
+  using substate_antisym by blast
+
+lemma constrained_always_einv2req: "
+(\<forall> s1. toEnvP s1 \<and> substate s1 s \<and> A s1 \<longrightarrow> A' s1) \<Longrightarrow>
+(\<forall> s1. toEnvP s1 \<and> substate s1 s \<and> constrained_always_inv s1 s t t1 A \<longrightarrow> constrained_always s1 s t A')"
+  apply(unfold constrained_always_inv_def constrained_always_def)
+  apply auto
+  done
+
+definition P5_2 where "P5_2 s t A1 A2 \<equiv>
+always2 s A1 (\<lambda> s2. constrained_always s2 s t A2)"
+
+definition P5_2inv where "P5_2inv s t t1 A1 A2 \<equiv>
+always2 s A1 (\<lambda> s2. constrained_always_inv s2 s t t1 A2)"
+
+lemma P5_2_rule: "consecutive s0 s \<Longrightarrow>
+P5_2inv s0 t t1 A1 A2 \<and> (\<not>A1 s0 s \<or> t = 0 \<or> t1' = 0 \<and> A2 s) \<and> (t1 + 1 \<ge> t \<or> A2 s) \<and> t1' \<le> t1 + 1 \<Longrightarrow>
+P5_2inv s t t1' A1 A2"
+  apply(unfold P5_2inv_def)
+(*  using always2_rule constrained_always_rule constrained_always_one_point
+  by (smt (verit))
+*)
+  apply(rule always2_rule[of s0])
+   apply simp
+  apply(rule conj_forward)
+    prefer 2
+    apply(rotate_tac -1)
+    apply assumption
+   prefer 2
+   apply(rule conj_forward)
+     prefer 2
+     apply(rule disj_forward)
+       prefer 2
+      apply(rotate_tac -1)
+       apply assumption
+      prefer 2
+      apply(rule constrained_always_one_point)
+    apply(rotate_tac -1)
+      apply assumption
+    apply(rotate_tac -1)
+     apply assumption
+    prefer 2
+    apply(rule constrained_always_rule[of s0])
+     apply simp
+    apply(rule disj_forward)
+      prefer 2
+    apply(rotate_tac -1)
+      apply assumption
+     prefer 2
+     apply(rule conj_forward)
+       prefer 2
+       apply(rule all_imp_refl)
+    apply(rotate_tac -1)
+       apply assumption
+      prefer 2
+      apply(rotate_tac -1)
+      apply assumption
+    apply(rotate_tac -1)
+     apply assumption
+    apply(rotate_tac -1)
+    apply assumption
+    apply(rotate_tac -1)
+   apply assumption
+  apply auto
+  done
+
+lemma P5_2_einv2req: " P5_2inv s t t1 A1 A2 \<Longrightarrow> P5_2 s t A1 A2"
+  apply(unfold P5_2inv_def P5_2_def)
+ (* using always2_einv2req constrained_always_einv2req
+  by (metis (no_types, lifting))
+*)
+  apply(rule always2_einv2req)
+  apply(rule conj_forward)
+    prefer 2
+    apply(rotate_tac -1)
+    apply assumption
+   prefer 2
+   apply(rule constrained_always_einv2req)
+   apply(rule all_imp_refl)
+   apply(rotate_tac -1)
+   apply assumption
+  apply auto
+  done
 
 end
-
