Patterns.thy
@@ -6,14 +6,9 @@ Pattern4_Def
 Pattern5_Def
 Pattern6_Def
 Pattern7_Def
-Pattern9_Def
 Pattern10_Def
 Pattern11_Def
 Pattern12_Def
 begin
-
-
-lemma imp_rule: "(A1 \<Longrightarrow> \<not>A1') \<Longrightarrow> (A2 \<Longrightarrow> A2') \<Longrightarrow> A1 \<or> A2 \<Longrightarrow> A1' \<longrightarrow> A2'"
-  by auto
 
 end
