SmartLighting/Proofs_R7.thy
@@ -1,0 +1,94 @@
+theory Proofs_R7
+  imports ExtraInv_R7_2 Requirements
+begin
+
+definition inv7 where "inv7 s \<equiv> extraInv s \<and> R7 s"
+
+theorem "VC1 inv7 s0"
+  apply(unfold VC1_def inv7_def R7_def P1_def)
+  using extra1 VC1_def apply auto
+  done
+
+theorem "VC148 inv7 env s0 motion_value light_value"
+  apply(unfold VC148_def inv7_def R7_def)
+  apply(rule impI)
+  apply(rule context_conjI)
+  using extra148 VC148_def apply auto[1]
+  apply(rule conjI)
+   apply simp
+  apply(unfold extraInv_def commonExtraInv_def)
+  apply(erule conjE)+
+  apply(auto simp add: Pattern1_Def.einv2req)
+  done
+
+theorem "VC166 inv7 env s0 motion_value light_value"
+  apply(unfold VC166_def inv7_def R7_def)
+  apply(rule impI)
+  apply(rule context_conjI)
+  using extra166 VC166_def apply auto[1]
+  apply(rule conjI)
+   apply simp
+  apply(unfold extraInv_def commonExtraInv_def)
+  apply(erule conjE)+
+  apply(auto simp add: Pattern1_Def.einv2req)
+  done
+
+theorem "VC184 inv7 env s0 motion_value light_value"
+  apply(unfold VC184_def inv7_def R7_def)
+  apply(rule impI)
+  apply(rule context_conjI)
+  using extra184 VC184_def apply auto[1]
+  apply(rule conjI)
+   apply simp
+  apply(unfold extraInv_def commonExtraInv_def)
+  apply(erule conjE)+
+  apply(auto simp add: Pattern1_Def.einv2req)
+  done
+
+theorem "VC202 inv7 env s0 motion_value light_value"
+  apply(unfold VC202_def inv7_def R7_def)
+  apply(rule impI)
+  apply(rule context_conjI)
+  using extra202 VC202_def apply auto[1]
+  apply(rule conjI)
+   apply simp
+  apply(unfold extraInv_def commonExtraInv_def)
+  apply(erule conjE)+
+  apply(auto simp add: Pattern1_Def.einv2req)
+  done
+
+theorem "VC238 inv7 env s0 motion_value light_value"
+  apply(unfold VC238_def inv7_def R7_def)
+  apply(rule impI)
+  apply(rule context_conjI)
+  using extra238 VC238_def apply auto[1]
+  apply(rule conjI)
+   apply simp
+  apply(unfold extraInv_def commonExtraInv_def)
+  apply(erule conjE)+
+  apply(auto simp add: Pattern1_Def.einv2req)
+  done
+
+theorem "VC256 inv7 env s0 motion_value light_value"
+  apply(unfold VC256_def inv7_def R7_def)
+  apply(rule impI)
+  apply(rule context_conjI)
+  using extra256 VC256_def apply auto[1]
+  apply(rule conjI)
+   apply simp
+  apply(unfold extraInv_def commonExtraInv_def)
+  apply(erule conjE)+
+  apply(auto simp add: Pattern1_Def.einv2req)
+  done
+
+theorem "VC274 inv7 env s0 motion_value light_value"
+  apply(unfold VC274_def inv7_def R7_def)
+  apply(rule impI)
+  apply(rule context_conjI)
+  using extra274 VC274_def apply auto[1]
+  apply(rule conjI)
+   apply simp
+  apply(unfold extraInv_def commonExtraInv_def)
+  apply(erule conjE)+
+  apply(auto simp add: Pattern1_Def.einv2req)
+  done
